platform/tests/Thread0.v
@@ -1,0 +1,17 @@
+Require Import Thread.
+Export Thread.
+
+
+Module M.
+  Definition globalInv : HProp := Emp%Sep.
+End M.
+
+Module T := Make(M).
+
+Import T.
+Export T.
+
+Notation sched := tq.
+
+Ltac sep hints := unfold M.globalInv in *; T.sep hints.
+Ltac sep_auto := sep auto_ext.
